Leansubst/Pointwise.lean
@@ -1,0 +1,107 @@
+import Leansubst.Basic
+
+/-!
+This file contains an alternative definition of variable substitution, and theorems
+establishing their equivalence with the parallel substitution defined in `Defs.lean`.
+
+If your definition of substitution more closely resembles the following,
+it can be easier to prove the required lemmas based on the results below.
+-/
+
+namespace Leansubst.Pointwise
+
+variable {σ : Type}
+
+/-!
+A [common definition](https://en.wikipedia.org/wiki/De_Bruijn_index#Formal_definition)
+of pointwise substitutions.
+-/
+
+/-- Shift variables with level ≥ `n` by `m` levels. -/
+def shift : Nat → Nat → Expr σ → Expr σ
+  | n, m, .var i     => if n <= i then .var (i + m) else .var i
+  | n, m, .binder e  => .binder (shift (n + 1) m e)
+  | n, m, .node x es => .node x (nested n m es)
+where nested : Nat → Nat → List (Expr σ) → List (Expr σ)
+  | _, _, []      => []
+  | n, m, e :: es => shift n m e :: nested n m es
+
+/-- Replace all variables at level = `n` by an expression `t`,
+    while decrementing all variables at level > `n`. -/
+def subst : Nat → Expr σ → Expr σ → Expr σ
+  | n, t, .var i     => if n < i then .var (.pred i) else if n = i then shift 0 n t else .var i
+  | n, t, .binder e  => .binder (subst (n + 1) t e)
+  | n, t, .node x es => .node x (nested n t es)
+where nested : Nat → Expr σ → List (Expr σ) → List (Expr σ)
+  | _, _, []      => []
+  | n, t, e :: es => subst n t e :: nested n t es
+
+/-- `Pointwise.shift n m` agrees with `Subst.apply (Subst.up n (Subst.shift m))`. -/
+@[simp]
+theorem shift_to_parallel (n m) : shift n m = Subst.apply (Subst.up n (Subst.shift σ m)) := by
+  apply funext; intros e;
+  -- Induction on `e`.
+  let motive := fun (e : Expr σ) => ∀ n m, shift n m e = Subst.apply (Subst.up n (Subst.shift σ m)) e
+  apply @Expr.recOn _ (fun e => motive e) (List.foldr (fun e etc => motive e ∧ etc) True)
+    <;> intros <;> (try trivial) <;> intros n m
+  case var i =>
+    rw [shift, Subst.apply]
+    split
+    case inl h =>
+      have ⟨d, hd⟩ := Nat.le.dest h; subst hd; clear h
+      rw [Subst.up_get_high, Subst.shift, Subst.applyr, Nat.add_assoc, Nat.add_comm, Nat.add_assoc]
+    case inr h =>
+      have h' := Nat.lt_of_not_le h; clear h
+      rw [Subst.up_get_low]; exact h'
+  case binder e ih => rw [shift, Subst.apply, Subst.up_up, ih]
+  case node x es ih =>
+    induction es with
+    | nil => simp only [shift, shift.nested, Subst.apply, Subst.apply.nested]
+    | cons h' t' ih' =>
+      rw [List.foldr] at ih
+      simp only [shift, shift.nested, Subst.apply, Subst.apply.nested] at *
+      congr 2
+      . exact ih.left _ _
+      . specialize ih' ih.right
+        simp only [shift, shift.nested, Subst.apply, Subst.apply.nested] at ih'
+        injection ih'
+
+/-- `Pointwise.subst n t` agrees with `Subst.apply (Subst.pointwise n t)`. -/
+@[simp]
+theorem subst_to_parallel (n t) : @subst σ n t = Subst.apply (Subst.pointwise n t) := by
+  apply funext; intros e;
+  -- Induction on `e`.
+  let motive := fun (e : Expr σ) => ∀ n t, @subst σ n t e = Subst.apply (Subst.pointwise n t) e
+  apply @Expr.recOn _ (fun e => motive e) (List.foldr (fun e etc => motive e ∧ etc) True)
+    <;> intros <;> (try trivial) <;> intros n t
+  case var i =>
+    rw [subst, Subst.pointwise, Subst.id, Subst.apply]
+    split <;> try split
+    case inl h =>
+      cases i with
+      | zero => contradiction
+      | succ i =>
+        have h' := Nat.le_of_lt_succ h; clear h
+        have ⟨d, hd⟩ := Nat.le.dest h'; subst hd; clear h'
+        rw [Nat.pred_succ, ← Nat.add_succ, Subst.up_get_high, Subst.cons, Subst.applyr, Nat.add_comm]
+    case inr.inl h₁ h₂ =>
+      subst h₂; clear h₁
+      conv => rhs; rhs; rw [← Nat.add_zero n]
+      rw [Subst.up_get_high, Subst.cons, Subst.applyr_to_apply, shift_to_parallel 0]; rfl
+    case inr.inr h₁ h₂ =>
+      have h := Nat.lt_of_le_of_ne (Nat.le_of_not_lt h₁) (Ne.symm h₂); clear h₁ h₂
+      rw [Subst.up_get_low]; exact h
+  case binder e ih => rw [subst, Subst.apply, ih]; rfl
+  case node x es ih =>
+    induction es with
+    | nil => simp only [subst, subst.nested, Subst.apply, Subst.apply.nested]
+    | cons h' t' ih' =>
+      rw [List.foldr] at ih
+      simp only [subst, subst.nested, Subst.apply, Subst.apply.nested] at *
+      congr 2
+      . exact ih.left _ _
+      . specialize ih' ih.right
+        simp only [subst, subst.nested, Subst.apply, Subst.apply.nested] at ih'
+        injection ih'
+
+end Leansubst.Pointwise
