README.md
@@ -1,13 +1,47 @@
 # Leansubst
 
-> This is still in very early stage and is definitely not as feature-complete as [Autosubst](https://github.com/coq-community/autosubst/). Rough implementation details can be seen everywhere. Renamings are not specially handled. Normalisation involving `shift`s and `up`s can get halfway stuck.
+Leansubst is a library for the [Lean theorem prover](https://leanprover.github.io/) which provides basic automation for formalising syntactic theories with variable binders.
+
+Given:
+
+1. An **injective map** from arbitrary user-defined syntactic object type to `Leansubst.Expr`,
+2. A proof that some user-defined substitution operation **agrees with** `Leansubst.Subst.apply`,
+
+the `@[simp]` lemmas supplied by Leansubst will be able to automatically prove some simple facts about substitutions.
+
+> ⚠ This is still in very early stage and is definitely not as feature-complete as [Autosubst](https://github.com/coq-community/autosubst/). Rough implementation details can be seen everywhere. Renamings are not specially handled. Normalisation involving `shift`s and `up`s can get halfway stuck.
+
+## Installation
+
+Add the following lines to the `lakefile.lean` file of your Lean 4 project:
+
+```lean
+require leansubst from git
+  "https://github.com/bridgekat/leansubst" @ "main" -- Or replace "main" with a fixed commit hash
+```
+
+and run `lake update` in the same directory.
 
 ## How to use
 
-See [`Examples.lean`](Leansubst/Examples.lean) (this will be simplified soon...)
+- See [`Examples.lean`](Leansubst/Examples.lean) for using Leansubst on a simple λ-calculus with pointwise substitutions defined.
+- For the definitions used by Leansubst, see [`Defs.lean`](Leansubst/Defs.lean) and [`Pointwise.lean`](Leansubst/Pointwise.lean).
+- For theorems and explanations, see the comments in [`Basic.lean`](Leansubst/Basic.lean).
 
-For definitions and explanations, see [`Defs.lean`](Leansubst/Defs.lean) and [`Basic.lean`](Leansubst/Basic.lean).
+```lean
+-- ... (User-supplied proof for `to_expr_inj`, `to_expr_shift` and `to_expr_subst`)
 
-There is plan to formalise the completeness and decidability proofs[^1] of the equational theory.
+example (s) :
+    .lam "x" (.app (.var 0) (.var 3)) ⟦2 ↦ s⟧ =
+    .lam "x" (.app (.var 0) (s ⟦0 ↟ 3⟧)) := by
+  apply to_expr_inj -- Start by turning the problem into one that Leansubst can recognise.
+  leansubst         -- Normalise!
+```
+
+There is also some plan to formalise the completeness and decidability proofs[^1] of the equational theory.
+
+## Bug reports
+
+Please submit bugs reports on [https://github.com/bridgekat/leansubst/issues](https://github.com/bridgekat/leansubst/issues).
 
 [^1]: [Completeness and Decidability of de Bruijn Substitution Algebra in Coq](https://www.ps.uni-saarland.de/Publications/documents/SchaeferEtAl_2015_Completeness.pdf) doi: [10.1145/2676724.2693163](https://doi.org/10.1145/2676724.2693163)
